ulib/FStar.HyperStack.All.fst
@@ -17,7 +17,7 @@ module FStar.HyperStack.All
 include FStar.HyperStack.ST
 
 let all_pre = all_pre_h HyperStack.mem
-let all_post' (a:Type) (pre:Type) = all_post_h' HyperStack.mem a pre
+let all_post' (a:Type) (pre:prop) = all_post_h' HyperStack.mem a pre
 let all_post  (a:Type) = all_post_h HyperStack.mem a
 let all_wp (a:Type) = all_wp_h HyperStack.mem a
 new_effect ALL = ALL_h HyperStack.mem
