ulib/FStar.Monotonic.Map.fst
@@ -12,7 +12,7 @@ type map' (a:Type) (b:a -> Type) =
   f:(x:a -> Tot (option (b x)))
 
 (* Partial, dependent maps, with a whole-map invariant *)
-type map (a:Type) (b:a -> Type) (inv:map' a b -> Type0) =
+type map (a:Type) (b:a -> Type) (inv:map' a b -> prop) =
   m:map' a b{inv m}
 
 let upd (#a:eqtype) #b (m:map' a b) (x:a) (y:b x)
@@ -46,11 +46,11 @@ let alloc (#r:rid) #a #b #inv
   = ralloc r (empty_map a b)
 
 let defined #r #a #b #inv (m:t r a b inv) (x:a) (h:HS.mem)
-  : GTot Type0
+  : GTot prop
   = Some? (sel (HS.sel h m) x)
 
 let contains #r #a #b #inv (m:t r a b inv) (x:a) (y:b x) (h:HS.mem)
-  : GTot Type0
+  : GTot prop
   = Some? (sel (HS.sel h m) x) /\ Some?.v (sel (HS.sel h m) x) == y
 
 let value #r #a #b #inv (m:t r a b inv) (x:a) (h:HS.mem{defined m x h})
@@ -58,14 +58,14 @@ let value #r #a #b #inv (m:t r a b inv) (x:a) (h:HS.mem{defined m x h})
   = Some?.v (sel (HS.sel h m) x)
 
 let fresh #r #a #b #inv (m:t r a b inv) (x:a) (h:HS.mem)
-  : GTot Type0
+  : GTot prop
   = None? (sel (HS.sel h m) x)
 
 let contains_stable #r #a #b #inv (m:t r a b inv) (x:a) (y:b x)
   : Lemma (ensures (stable_on_t m (contains m x y)))
   = ()
 
-let extend (#r:rid) (#a:eqtype) (#b:a -> Type) (#inv:(map' a b -> Type0)) (m:t r a b inv) (x:a) (y:b x)
+let extend (#r:rid) (#a:eqtype) (#b:a -> Type) (#inv:(map' a b -> prop)) (m:t r a b inv) (x:a) (y:b x)
   : ST unit
       (requires (fun h -> let cur = HS.sel h m in inv (upd cur x y) /\ sel cur x == None))
       (ensures (fun h0 u h1 ->
